last commit before removing bijection

theories/stacked_borrows/heap.v
@@ -68,6 +68,92 @@ Fixpoint active_SRO (stk: stack) : gset ptr_id :=
   end.
 
 
+Fixpoint heap_array (l : loc) (scs : list scalar) : gmap loc scalar :=
+  match scs with
+  | [] => ∅
+  | sc :: scs' => {[l := sc]} ∪ heap_array (l +ₗ 1) scs'
+  end.
+
+Lemma heap_array_singleton l sc : heap_array l [sc] = {[l := sc]}.
+Proof. by rewrite /heap_array right_id. Qed.
+
+Lemma heap_array_lookup l scs sc k :
+  heap_array l scs !! k = Some sc ↔
+  ∃ j, (0 ≤ j)%Z ∧ k = l +ₗ j ∧ scs !! (Z.to_nat j) = Some sc.
+Proof.
+  revert k l; induction scs as [|sc' scs IH]=> l' l /=.
+  { rewrite lookup_empty. naive_solver lia. }
+  rewrite -insert_union_singleton_l lookup_insert_Some IH. split.
+  - intros [[-> ->] | (Hl & j & ? & -> & ?)].
+    { eexists 0. rewrite shift_loc_0. naive_solver lia. }
+    eexists (1 + j)%Z. rewrite shift_loc_assoc !Z.add_1_l Z2Nat.inj_succ; auto with lia.
+  - intros (j & ? & -> & Hil). destruct (decide (j = 0)); simplify_eq/=.
+    { rewrite shift_loc_0; eauto. }
+    right. split.
+    { rewrite -{1}(shift_loc_0 l). intros ?%(inj (shift_loc _)); lia. }
+    assert (Z.to_nat j = S (Z.to_nat (j - 1))) as Hj.
+    { rewrite -Z2Nat.inj_succ; last lia. f_equal; lia. }
+    rewrite Hj /= in Hil.
+    eexists (j - 1)%Z. rewrite shift_loc_assoc Z.add_sub_assoc Z.add_simpl_l.
+    auto with lia.
+Qed.
+
+Lemma heap_array_map_disjoint (h : gmap loc scalar) (l : loc) (scs : list scalar) :
+  (∀ i, (0 ≤ i)%Z → (i < length scs)%Z → h !! (l +ₗ i) = None) →
+  (heap_array l scs) ##ₘ h.
+Proof.
+  intros Hdisj. apply map_disjoint_spec=> l' v1 v2.
+  intros (j&?&->&Hj%lookup_lt_Some%inj_lt)%heap_array_lookup.
+  move: Hj. rewrite Z2Nat.id // => ?. by rewrite Hdisj.
+Qed.
+
+Lemma lookup_free_mem_1 l l' n σ :
+  l.1 ≠ l'.1 → (free_mem l n σ) !! l' = σ !! l'.
+Proof.
+  induction n as [ | n IH] in l |-*; cbn; first done.
+  intros Hneq. rewrite lookup_delete_ne; last by congruence.
+  by apply IH.
+Qed.
+Lemma lookup_free_mem_2 l l' (n : nat) σ :
+  l.1 = l'.1 → (l.2 ≤ l'.2 < l.2 + n)%Z → (free_mem l n σ) !! l' = None.
+Proof.
+  induction n as [ | n IH] in l |-*; cbn; first lia.
+  intros Hchunk Hi.
+  destruct (decide (l.2 = l'.2)) as [Heq | Hneq].
+  - rewrite lookup_delete_None; left. destruct l, l'; simpl in *; congruence.
+  - rewrite lookup_delete_ne; last congruence. apply IH; first done. destruct l, l'; simpl in *; lia.
+Qed.
+Lemma lookup_free_mem_3 l l' (n : nat) σ :
+  l.1 = l'.1 → (l'.2 < l.2)%Z → (free_mem l n σ) !! l' = σ !! l'.
+Proof.
+  induction n as [ | n IH] in l |-*; cbn; first done.
+  intros Hchunk Hi. rewrite lookup_delete_ne.
+  - apply IH; first done. destruct l, l'; cbn in *; lia.
+  - destruct l, l'; cbn in *; intros [=]. lia.
+Qed.
+Lemma lookup_free_mem_4 l l' (n : nat) σ :
+  l.1 = l'.1 → (l'.2 >= l.2 + n)%Z → (free_mem l n σ) !! l' = σ !! l'.
+Proof.
+  induction n as [ | n IH] in l |-*; cbn; first done.
+  intros Hchunk Hi. rewrite lookup_delete_ne.
+  - apply IH; first done. destruct l, l'; cbn in *; lia.
+  - destruct l, l'; cbn in *; intros [=]. lia.
+Qed.
+
+Lemma delete_free_mem σ l n o:
+  (o > 0)%Z →
+  delete l (free_mem (l +ₗ o) n σ) = free_mem (l +ₗ o) n (delete l σ).
+Proof.
+  intros HO.
+  induction n as [|n IH] in o, HO|-* => //=. rewrite delete_commute. f_equal.
+  rewrite shift_loc_assoc IH; [done | lia].
+Qed.
+
+Definition state_upd_mem (f : mem → mem) σ :=
+  mkState (f σ.(shp)) σ.(sst) σ.(scs) σ.(snp) σ.(snc).
+Definition state_upd_stacks (f : stacks → stacks) σ :=
+  mkState σ.(shp) (f σ.(sst)) σ.(scs) σ.(snp) σ.(snc).
+
 
 
 (* maintain for each tag: the permissions (public or unique) and, optionally, the
@@ -79,9 +165,14 @@ Class bor_stateG Σ := {
   (*heap_source_name : gname;*)
   (*heap_target_name : gname;*)
 
-  (* A bijection on blocks, stating the size of the allocation and that the stacks are pointwise the same *)
-  (*heap_bij_inG :> gset_bijG Σ block block;*)
-  (*heap_bij_name : gname;*)
+  (* A bijection on blocks, stating that the size of the allocation and the stacks are pointwise the same, and the target locations are in public or private relation *)
+  heap_bij_inG :> gset_bijG Σ block block;
+  heap_bij_name : gname;
+
+  (* Size of blocks *)
+  freeable_inG :> ghost_mapG Σ loc (option nat);
+  freeable_source_name : gname;
+  freeable_target_name : gname;
 
   (* Maintaining the locations protected by each call id *)
   call_inG :> ghost_mapG Σ call_id (gmap ptr_id (gset loc));
@@ -89,7 +180,7 @@ Class bor_stateG Σ := {
   call_target_name : gname;
 
   (* tag ownership *)
-  tag_inG :> tkmapG Σ ptr_id (option unit);
+  tag_inG :> tkmapG Σ ptr_id unit;
   tag_name : gname;
 
   (* A view of parts of the heap, conditional on the ptr_id *)
@@ -98,24 +189,279 @@ Class bor_stateG Σ := {
   heap_view_target_name : gname;
 }.
 
-(* Interpretation for "local" fragments of the heap *)
-(*Section loc_heap_defs.*)
-  (*Context {Σ} (heap_gname : gname) {heap_inG : ghost_mapG Σ loc (scalar * stack)}.*)
+(* NOTE: doing this in simplang style doesn't work. 
+  the language doesn't offer any guarantees that locations that were used once will not be re-used.
+ *)
+Section freeable.
+  Context {Σ} (freeable_name : gname) {freeable_inG : ghost_mapG Σ loc (option nat)}.
+  (*[σ] is the heap map. [bs] is the set of all blocks ever allocated. [hF] is the freeable map, mapping to the allocation size. *)
+  Definition heap_freeable_rel (σ : gmap loc scalar) (bs : gset block) (hF : gmap loc (option nat)) : Prop :=
+    ∀ l (o : option nat), hF !! l = Some o →
+     l.1 ∈ bs ∧
+     l.2 = 0 ∧
+     0 < default 1%nat o ∧
+     ∀ i, is_Some (σ !! (l +ₗ i)) ↔ (0 ≤ i < default O o)%Z.
 
-  (*Definition heap_pointsto (l : loc) (sc : scalar)  (s : stack) :=*)
-    (*ghost_map_elem heap_gname l (DfracOwn 1) (sc, s).*)
+  Definition heap_freeable_def (l : loc) (q : Qp) (n: option nat) : iProp Σ :=
+    ⌜l.2 = 0⌝ ∗ l ↪[ freeable_name ]{# q } n.
+  Definition heap_freeable_aux : seal (@heap_freeable_def). by eexists. Qed.
+  Definition heap_freeable := unseal heap_freeable_aux.
+  Definition heap_freeable_eq : @heap_freeable = @heap_freeable_def :=
+    seal_eq heap_freeable_aux.
 
-  (*Definition heap_interp (σ : state) : iProp Σ := *)
-    (*∃ M : gmap loc (scalar * stack), ghost_map_auth heap_gname 1 M ∗*)
-      (*⌜∀ l sc s, M !! l = Some (sc, s) → σ.(shp) !! l = Some sc ∧ σ.(sst) !! l = Some s⌝.*)
+  Definition heap_freeable_auth σ bs : iProp Σ := ∃ hF,
+    ghost_map_auth freeable_name 1 hF ∗ ⌜heap_freeable_rel σ bs hF⌝.
+
+  Local Notation "†{ q } l …? n" := (heap_freeable l q n)
+  (at level 20, q at level 50, format "†{ q } l …? n") : bi_scope.
+  Local Notation "† l …? n" := (heap_freeable  l 1 n) (at level 20) : bi_scope.
+
+  Lemma heap_freeable_idx l n :
+    †l…?n -∗ ⌜l.2 = 0⌝.
+  Proof. rewrite heap_freeable_eq. iIntros "[$ _]". Qed.
+
+  Lemma heap_freeable_excl l l' n n' :
+    l.1 = l'.1 →
+    †l…?n -∗ †l'…?n' -∗ False.
+  Proof.
+    rewrite heap_freeable_eq.
+    iIntros (?) "[% Hl1] [% Hl2]". destruct l, l'; simplify_eq/=.
+    by iDestruct (ghost_map_elem_valid_2 with "Hl1 Hl2") as %[? ?].
+  Qed.
+
+  Lemma heap_freeable_rel_stable σ bs h l p :
+    heap_freeable_rel σ bs h → is_Some (σ !! l) →
+    heap_freeable_rel (<[l := p]>σ) bs h.
+  Proof.
+    intros REL Hσ blk qs Hqs. destruct (REL blk qs) as [? [? [? REL']]]; first done.
+    split_and!; [done..|]=> i. rewrite -REL' lookup_insert_is_Some.
+    destruct (decide (l = blk +ₗ i)); naive_solver.
+  Qed.
+
+  Instance option_proper A : Proper ((=) ==> iff) (is_Some (A:=A)). 
+  Proof. intros a b ->; done. Qed.
+
+  Lemma heap_freeable_rel_init_mem l h n σ bs sc:
+    n ≠ O →
+    l.2 = 0 →
+    l.1 ∉ bs →
+    (∀ m : Z, σ !! (l +ₗ m) = None) →
+    heap_freeable_rel σ bs h →
+    heap_freeable_rel (heap_array l (replicate n sc) ∪ σ) ({[l.1]} ∪ bs)
+                      (<[l := Some n]> h).
+  Proof.
+    move => ?? Hnotin Hnone Hrel l' o /lookup_insert_Some[[??]|[? Hl]]; simplify_eq/=.
+    - split_and!; [set_solver|done|lia|] => i.
+      split.
+      + move => [?].
+        rewrite lookup_union_Some ?Hnone.
+        2: { apply heap_array_map_disjoint. naive_solver lia. }
+        rewrite heap_array_lookup => -[[?[?[?]]]|//]. simplify_eq.
+        rewrite lookup_replicate. lia.
+      + move => ?.
+        eexists _.
+        rewrite lookup_union_Some ?Hnone.
+        2: { apply heap_array_map_disjoint. naive_solver lia. }
+        left. apply heap_array_lookup. eexists i.
+        split_and!; [lia|done |].
+        rewrite lookup_replicate. naive_solver lia.
+    - have [?[?[? Hi]]]:= Hrel _ _ Hl.
+      split_and!; [set_solver|done|lia|] => i.
+      have <-:= Hi i. f_equiv.
+      apply option_eq => ?.
+      rewrite lookup_union_Some.
+      2: { apply heap_array_map_disjoint. naive_solver lia. }
+      rewrite heap_array_lookup.
+      split; [|naive_solver].
+      move => [[?[?[?]]]|//].
+      contradict Hnotin.
+      have ->: l.1 = l'.1 by destruct l, l'; naive_solver.
+      done.
+  Qed.
+
+  Lemma heap_freeable_rel_free_mem σ hF n l bs:
+    l.2 = 0 →
+    hF !! l = Some (Some n) →
+    heap_freeable_rel σ bs hF →
+    heap_freeable_rel (free_mem l n σ) bs (<[l:=None]> hF).
+  Proof.
+    intros ? Hl REL b qs Hlookup.
+    destruct (REL l (Some n)) as [? [? [? REL']]]; auto.
+    move: Hlookup => /lookup_insert_Some [[??]|[NEQ ?]]; simplify_eq.
+    - split_and!; [done| done| simpl; lia |] => i /=. split; [|lia] => -[?].
+      have ->: free_mem b n σ !! (b +ₗ i) = None; last naive_solver.
+      destruct (decide (0 ≤ i < n))%Z.
+      + apply lookup_free_mem_2; [done|]. simpl. lia.
+      + destruct (decide (i < 0))%Z.
+        * rewrite lookup_free_mem_3 => /=; [|done|lia].
+          apply eq_None_not_Some. naive_solver lia.
+        * rewrite lookup_free_mem_4 => /=; [|done|lia].
+          apply eq_None_not_Some. naive_solver lia.
+    - destruct (REL b qs) as [? [? [? REL'']]]; auto.
+      split_and!; [done..|]=> i. rewrite -REL'' lookup_free_mem_1 //=.
+      destruct b, l; simplify_eq/=. congruence.
+  Qed.
+
+  (*Lemma heap_freeable_inj n1 l1 l2 n2 σ bs:*)
+    (*(0 < n1)%Z →*)
+    (*(∀ m, is_Some (σ !! (l1 +ₗ m)) ↔ (0 ≤ m < n1)%Z) →*)
+    (*loc_chunk l1 = loc_chunk l2 →*)
+    (*heap_ctx γ σ bs -∗ †l2…?n2 -∗ ⌜n2 = Some (Z.to_nat n1) ∧ l1 = l2⌝.*)
+  (*Proof.*)
+    (*iIntros (? Hrel1 ?) "(%hF & ? & HhF & %Hrel) Hf".*)
+    (*rewrite heap_freeable_eq. iDestruct "Hf" as (?) "Hf".*)
+    (*iDestruct (ghost_map_lookup with "HhF Hf") as %Hf.*)
+    (*iPureIntro.*)
+    (*have [? [? [? {}Hrel2]]]:= Hrel _ _ Hf.*)
+    (*destruct n2; last first. {*)
+      (*have [_ [|? Hl]]:= Hrel1 0; [lia|].*)
+      (*have [/=[|] ]:= Hrel2 (loc_idx l1 - loc_idx l2)%Z; last lia.*)
+      (*eexists _. erewrite <-Hl. f_equal. rewrite /loc_add. destruct l1, l2 => /=.*)
+      (*f_equal; [done |lia].*)
+    (*}*)
+    (*simplify_eq/=.*)
+    (*destruct (decide (l1 = l2)).*)
+    (*{ subst. split; [|done].*)
+      (*have Heq: (∀ i : Z, (0 ≤ i < n) ↔ (0 ≤ i < n1))%Z. naive_solver.*)
+      (*f_equal.*)
+      (*destruct (decide (n1 < n)%Z). { have := Heq n1. lia. }*)
+      (*destruct (decide (n < n1)%Z). { have := Heq n. lia. }*)
+      (*lia.*)
+    (*}*)
+    (*have ?: loc_idx l1 ≠ loc_idx l2 by destruct l1, l2;  naive_solver.*)
+    (*destruct (decide (loc_idx l1 < loc_idx l2)%Z).*)
+    (*- have [_ [|? Hl]]:= Hrel1 0; first lia.*)
+      (*have [/=[|] ]:= Hrel2 (loc_idx l1 - loc_idx l2)%Z; last lia.*)
+      (*eexists _. erewrite <-Hl. f_equal. rewrite /loc_add. destruct l1, l2 => /=.*)
+      (*f_equal; [done |lia].*)
+    (*- have [_ [|? Hl]]:= Hrel2 0; first lia.*)
+      (*have [/=[|] ]:= Hrel1 (loc_idx l2 - loc_idx l1)%Z; last lia.*)
+      (*eexists _. erewrite <-Hl. f_equal. rewrite /loc_add. destruct l1, l2 => /=.*)
+      (*f_equal; [done |lia].*)
+  (*Qed.*)
+
+  (*Lemma heap_freeable_lookup σ l l' x n bs:*)
+    (*σ !! l' = Some x → loc_chunk l' = loc_chunk l →*)
+    (*heap_ctx γ σ bs -∗ †l…?n -∗ ⌜∃ n' : nat, n' < default 0 n ∧ l' = l +ₗ n'⌝.*)
+  (*Proof.*)
+    (*iIntros (Hlo ?) "(%hF&?&HhF&%Hrel) Hf".*)
+    (*rewrite heap_freeable_eq. iDestruct "Hf" as (?) "Hf".*)
+    (*iDestruct (ghost_map_lookup with "HhF Hf") as %Hf.*)
+    (*iPureIntro.*)
+    (*have [? {}Hrel]:= Hrel _ _ Hf.*)
+    (*have Hl': l' = (l +ₗ (loc_idx l' - loc_idx l)).*)
+    (*{ destruct l', l => /=. rewrite /loc_add/=. f_equal; [done|lia]. }*)
+    (*rewrite Hl' in Hlo.*)
+    (*eapply mk_is_Some, Hrel in Hlo.*)
+    (*eexists (Z.to_nat (loc_idx l' - loc_idx l)). split; [lia|].*)
+    (*rewrite Hl'. f_equal => /=. lia.*)
+  (*Qed.*)
+End freeable.
+
+(** Allocation size notation *)
+Notation "† l '…?t' n" := (heap_freeable freeable_target_name l 1 n)
+  (at level 20, format "† l …?t  n") : bi_scope.
+Notation "† l '…t' n" := (heap_freeable freeable_target_name l 1 (Some n))
+  (at level 20, format "† l …t  n") : bi_scope.
+Notation "† l '…t' -" := (heap_freeable freeable_target_name l 1 None)
+  (at level 20, format "† l …t  -") : bi_scope.
+Notation "† l '…?s' n" := (heap_freeable freeable_source_name l 1 n)
+  (at level 20, format "† l …?s  n") : bi_scope.
+Notation "† l '…s' n" := (heap_freeable freeable_source_name l 1 (Some n))
+  (at level 20, format "† l …s  n") : bi_scope.
+Notation "† l '…s' -" := (heap_freeable freeable_source_name l 1 None)
+  (at level 20, format "† l …s  -") : bi_scope.
 
 
-(*End loc_heap_defs.*)
+Section mem_bijection.
+  Context {Σ} `{bor_stateG Σ}.
 
-(*Notation "l '↦t' sct" := (heap_pointsto heap_target_name l sct.1 sct.2)*)
-  (*(at level 20, format "l  ↦t sct") : bi_scope.*)
-(*Notation "l '↦s' sct" := (heap_pointsto heap_source_name l sct.1 sct.2)*)
-  (*(at level 20, format "l  ↦s sct") : bi_scope.*)
+  Definition heap_bij_auth (L : gset (block * block)) : iProp Σ :=
+    gset_bij_own_auth heap_bij_name (DfracOwn 1) L.
+  Definition heap_bij_elem (b_t : block) (b_s : block) :=
+    gset_bij_own_elem heap_bij_name b_t b_s.
+  Definition heap_bij_elem_loc (l_t l_s : loc) : iProp Σ :=
+    heap_bij_elem l_t.1 l_s.1 ∗ ⌜l_t.2 = l_s.2⌝.
+
+  (* The bijection serves the following purpose:
+      * the blocks are of the same size
+      * the stacks for the locations are pointwise the same
+      * every location is either a private location or a public location, which is tied to the tag ghost state 
+  *)
+  Context (sc_rel : scalar → scalar → iProp Σ).
+
+  Section defs.
+  (* We need all the maps from the tag interpretation here....
+     TODO: can we make that more beautiful? all the different invariants are interleaved in subtle ways, which makes modular reasoning really hard... *)
+    Context (M_tag : gmap ptr_id (tag_kind * unit)) (M_t M_s : gmap (ptr_id * loc) scalar) (Mcall_t : gmap call_id (gmap ptr_id (gset loc))).
+
+    Definition pub_loc σ_t σ_s (l_t l_s : loc) : iProp Σ := 
+      ∀ sc_t, ⌜σ_t.(shp) !! l_t = Some sc_t⌝ → ∃ sc_s, ⌜σ_s.(shp) !! l_s = Some sc_s⌝ ∗ sc_rel sc_t sc_s.
+    Definition priv_loc t (l_t : loc) : Prop := 
+      ∃ tk, M_tag !! t = Some (tk, tt) ∧ is_Some (M_t !! (t, l_t)) ∧
+        (* local *)
+        (tk = tk_local ∨ 
+        (* unique with protector *)
+        (tk = tk_unq ∧ ∃ c M' L, Mcall_t !! c = Some M' ∧ M' !! t = Some L ∧ l_t ∈ L)).
+      
+    Definition alloc_block_rel (σ_t σ_s : state) (b_t b_s : block) : iProp Σ :=  
+      ∃ n : option nat, 
+        (* same size *)
+        † (b_t, 0) …?t n ∗ † (b_s, 0) …?s n ∗
+        (* same stacks *)
+        ⌜∀ i st, σ_t.(sst) !! (b_t, i) = Some st → σ_s.(sst) !! (b_s, i) = Some st⌝ ∗
+        (* private / public locations of the target *)
+        ∀ i, ⌜is_Some (σ_t.(shp) !! (b_t, i))⌝ → 
+          pub_loc σ_t σ_s (b_t, i) (b_s, i) ∨ ⌜∃ t, priv_loc t (b_t, i)⌝.
+
+    Definition heap_bij_interp (L : gset (block * block)) σ_t σ_s : iProp Σ :=
+      [∗ set] p ∈ L, let '(b_t, b_s) := p in alloc_block_rel σ_t σ_s b_t b_s.
+  End defs.
+End mem_bijection.
+
+Notation "b_t '⇔h' b_s" := (heap_bij_elem b_t b_s) (at level 50) : bi_scope. 
+Notation "l_t '↔h' l_s" := (heap_bij_elem_loc l_t l_s) (at level 50) : bi_scope.
+
+Section bijection_lemmas.
+  Context {Σ} `{bor_stateG Σ}.
+  Context (sc_rel : scalar → scalar → iProp Σ).
+
+  (*Lemma heap_bij_interp_alloc L t : *)
+    (*(∀ b_s, (b_t, b_s) ∉ L) →*)
+    (*heap_bij_interp sc_rel M_tag M_t Mcall_t L σ_t σ_s -∗*)
+    (*heap_bij_interp sc_rel M_tag (Minit_mem ) Mcall_t L (state_upd_mem (init_mem (b_t, 0) n) σ_t)*)
+
+
+  (* TODO: accessors *)
+  Lemma heap_bij_interp_update_private_target M_tag M_t Mcall_t L σ_t σ_s l_t t sc : 
+    is_Some (σ_t.(shp) !! l_t) →
+    priv_loc M_tag M_t Mcall_t t l_t →
+    heap_bij_interp sc_rel M_tag M_t Mcall_t L σ_t σ_s -∗
+    heap_bij_interp sc_rel M_tag (<[(t, l_t) := sc]> M_t) Mcall_t L (state_upd_mem (<[l_t := sc]>) σ_t) σ_s.
+  Proof.
+    (* 
+      1. CA: is the block in the bijection or not. If not, we are done.
+      2. Otherwise, the interesting part are the public/private locations.
+      3. We prove that it is a private location for t. 
+    *)
+  Admitted.
+
+  Lemma heap_bij_interp_update_private_source M_tag M_t Mcall_t L σ_t σ_s l_t l_s t sc : 
+    is_Some (σ_t.(shp) !! l_t) →
+    priv_loc M_tag M_t Mcall_t t l_t →
+    (l_t.1, l_s.1) ∈ L →
+    l_t.2 = l_s.2 → 
+    heap_bij_interp sc_rel M_tag M_t Mcall_t L σ_t σ_s -∗
+    heap_bij_interp sc_rel M_tag M_t Mcall_t L σ_t (state_upd_mem (<[l_s := sc]>) σ_s).
+  Proof.
+    (* 
+      1. the interesting part are the public/private locations.
+      2. We prove that the target location is private. 
+          For any other location, this is fine, because l_t is in bijection with l_s, 
+            so other locations cannot be tripped by that.
+    *)
+  Admitted.
+End bijection_lemmas.
 
 (* Interpretation for call ids *)
 Section call_defs.
@@ -128,33 +474,25 @@ Section call_defs.
 
   (* This does not assert ownership of the authoritative part. Instead, this is owned by bor_interp below, 
     since also the block bijection needs access to it. *)
-  Definition call_set_interp (M : gmap call_id (gmap ptr_id (gset loc))) (σ : state) : iProp Σ :=
-    ⌜∀ c (M' : gmap ptr_id (gset loc)), M !! c = Some M' →
+  Definition call_set_interp (M : gmap call_id (gmap ptr_id (gset loc))) (σ : state) : Prop :=
+    ∀ c (M' : gmap ptr_id (gset loc)), M !! c = Some M' →
       c ∈ σ.(scs) ∧
       (* for every ptr_id *)
       ∀ pid (S : gset loc), M' !! pid = Some S →
         pid < σ.(snp) ∧
         (* for every protected location [l], there needs to be a protector in the stack *)
         ∀ (l : loc), l ∈ S → ∃ s pm, σ.(sst) !! l = Some s ∧
-          mkItem pm (Tagged pid) (Some c) ∈ s ∧ pm ≠ Disabled⌝.
+          mkItem pm (Tagged pid) (Some c) ∈ s ∧ pm ≠ Disabled.
 End call_defs.
 
 Notation "c '@s@' M" := (call_set_is call_source_name c M) (at level 50).
 Notation "c '@t@' M" := (call_set_is call_target_name c M) (at level 50).
 
-Notation "p '-->[' tk ']' ol" := (tkmap_elem tag_name p tk ol) (at level 50).
-
-Definition state_upd_mem (f : mem → mem) σ :=
-  mkState (f σ.(shp)) σ.(sst) σ.(scs) σ.(snp) σ.(snc).
-Definition state_upd_stacks (f : stacks → stacks) σ :=
-  mkState σ.(shp) (f σ.(sst)) σ.(scs) σ.(snp) σ.(snc).
 
 (* Interpretation for heap assertions under control of tags
     The interpretation of the tag map and the "heap view" fragments are interlinked.
  *)
 Section heap_defs.
-  Context {Σ} (heap_gname_t heap_gname_s tag_name : gname) {tag_inG : tkmapG Σ ptr_id (option unit) } {heap_inG : ghost_mapG Σ (ptr_id * loc) scalar}.
-
   (** The assumption on the location still being valid for tag [t], i.e., [t] not being disabled. *)
   Definition bor_state_pre (l : loc) (t : ptr_id) (tk : tag_kind) (s : stack) :=
     tk = tk_local ∨ ∃ pm pro, mkItem pm (Tagged t) pro ∈ s ∧ pm ≠ Disabled.
@@ -166,10 +504,6 @@ Section heap_defs.
     (tk = tk_pub ∧ t ∈ active_SRO s) ∨
     (tk = tk_local ∧ s = [mkItem Unique (Tagged t) None]).
 
-  (* TODO: I think we will want to generalize this by not having these explicit ownership modes,
-      but rather having a disjunction "either the value in the ghost state is current, because there are only reading items on top, or it is not current and there are other writing items on top.
-      Then we could use the stack assertion to determine which case we are in and what behavior we get.
-  *)
   Definition loc_controlled (l : loc) (t : ptr_id) (tk : tag_kind) (sc : scalar) (σ : state) :=
     ∃ s, σ.(sst) !! l = Some s ∧
       (bor_state_pre l t tk s → bor_state_own l t tk s ∧ σ.(shp) !! l = Some sc).
@@ -233,36 +567,23 @@ Section heap_defs.
     (*rewrite lookup_insert; done. *)
   (*Qed.*)
 
-
-
-  (* TODO: probably need to incorporate here that the blocks are in bijection
-      i.e.: stacks are pointwise the same, length of blocks is the same.
-  *)
-  Context (sc_rel : scalar → scalar → iProp Σ).
-  Definition tag_interp (M : gmap ptr_id (tag_kind * option unit)) (M_t M_s : gmap (ptr_id * loc) scalar) σ_t σ_s : iProp Σ := 
-    ∀ (t : ptr_id) tk ol, ⌜M !! t = Some (tk, ol)⌝ -∗
+  Definition tag_interp (M : gmap ptr_id (tag_kind * unit)) (M_t M_s : gmap (ptr_id * loc) scalar) σ_t σ_s : Prop := 
+    ∀ (t : ptr_id) tk, M !! t = Some (tk, ()) → 
       (* tags are valid *)
-      ⌜(t < σ_t.(snp))%nat⌝ ∧ ⌜(t < σ_s.(snp))%nat⌝ ∗
-      (
-        (* tag allocated, but locations are currently not shared *)
-        (*⌜(ol = None ∧ ∀ l, M_t !! (t, l) = None ∧ M_s !! (t, l) = None)⌝ ∨*)
-      (* tag allocated and the locations are shared *)
-      (∃ lb_t lb_s (len : nat), ⌜ol = Some tt⌝ ∗
+      (t < σ_t.(snp))%nat ∧ (t < σ_s.(snp))%nat ∧
+      (∃ lb_t lb_s (len : nat),
         (* at all offsets, the values agree, and match the physical state assuming the tag currently has control over the location *)
-        (∀ o, ⌜o < len⌝ → ∃ sc_t sc_s,
-          ⌜M_t !! (t, lb_t +ₗ o) = Some sc_t ∧ loc_controlled (lb_t +ₗ o) t tk sc_t σ_t ∧
-          M_s !! (t, lb_s +ₗ o) = Some sc_s ∧ loc_controlled (lb_s +ₗ o) t tk sc_s σ_s⌝ ∗
-          (* values need to be related if the tag is public. TODO: remove *)
-          (⌜tk = tk_pub⌝ → sc_rel sc_t sc_s)) ∗
-        (* TODO: assert same size of allocation here *)
+        (∀ o, o < len → ∃ sc_t sc_s,
+          M_t !! (t, lb_t +ₗ o) = Some sc_t ∧ loc_controlled (lb_t +ₗ o) t tk sc_t σ_t ∧
+          M_s !! (t, lb_s +ₗ o) = Some sc_s ∧ loc_controlled (lb_s +ₗ o) t tk sc_s σ_s) ∧ 
         (* locations in the heap view are valid *)
-        (⌜∀ l sc, M_t !! (t, l) = Some sc → ∃ o : nat, l = lb_t +ₗ o ∧ o < len⌝) ∗
-        (⌜∀ l sc, M_s !! (t, l) = Some sc → ∃ o : nat, l = lb_s +ₗ o ∧ o < len⌝)
-      )).
-  Global Instance tag_interp_persistent M M_t M_s σ_t σ_s : 
-    (∀ sc_t sc_s, Persistent (sc_rel sc_t sc_s)) → Persistent (tag_interp M M_t M_s σ_t σ_s).
-  Proof. intros Hpers. apply _. Qed.
+        (∀ l sc, M_t !! (t, l) = Some sc → ∃ o : nat, l = lb_t +ₗ o ∧ o < len) ∧
+        (∀ l sc, M_s !! (t, l) = Some sc → ∃ o : nat, l = lb_s +ₗ o ∧ o < len)
+      ).
 End heap_defs.
+
+
+Notation "p '@@' tk" := (tkmap_elem tag_name p tk ()) (at level 50).
 
 Notation "l '↦t[unq]{' t } sc" := (ghost_map_elem heap_view_target_name (t, l) (DfracOwn 1) sc)
   (at level 20, format "l  ↦t[unq]{ t }  sc") : bi_scope.
@@ -278,62 +599,31 @@ Notation "l '↦s[pub]{' t } sc" := (ghost_map_elem heap_view_source_name (t, l)
   (at level 20, format "l  ↦s[pub]{ t }  sc") : bi_scope.
 
 
-(* TODO *)
-(*Section mem_bijection.*)
-  (*Context {Σ} (sbijG_bij_name : gname) {bij_inG : gset_bijG Σ block block}.*)
-
-  (*Definition heap_bij_auth (L : gset (block * block)) : iProp Σ :=*)
-    (*gset_bij_own_auth sbijG_bij_name (DfracOwn 1) L.*)
-  (*Definition heap_bij_elem (l_t : block) (l_s : block) :=*)
-    (*gset_bij_own_elem sbijG_bij_name l_t l_s.*)
-
-  (*Definition alloc_shr_rel val_rel b_t b_s pid : iProp Σ :=*)
-    (*(∃ n vs_t vs_s, *)
-      (*(Loc b_t 0, pid) ↦t∗{dq} map (λ v, (v, tk_shr)) vs_t ∗*)
-      (*(Loc b_s 0, pid) ↦s∗{dq} map (λ v, (v, tk_shr)) vs_s ∗*)
-      (*vrel_list val_rel vs_t vs_s ∗*)
-      (*⌜length vs_t = n ∧ length vs_s = n⌝ ∗*)
-      (*mkloc b_t 0 ==>t n ∗*)
-      (*mkloc b_s 0 ==>s n).*)
-
-  (*Definition alloc_unq_rel val_rel b_t b_s pid : iProp Σ :=*)
-    (*(∃ (n : nat) vs_t vs_s,*)
-      (*(Loc b_t 0, pid) ↦t∗ map (λ v, (v, tk_unq)) vs_t ∗*)
-      (*(Loc b_s 0, pid) ↦s∗ map (λ v, (v, tk_unq)) vs_s ∗*)
-      (*vrel_list val_rel vs_t vs_s ∗*)
-      (*⌜length vs_t = n ∧ length vs_s = n⌝ ∗*)
-      (*mkloc b_t 0 ==>t n ∗*)
-      (*mkloc b_s 0 ==>s n).*)
-
-  (*Definition heap_bij_interp (val_rel : val → val → iProp Σ) :=*)
-    (*(∃ L, heap_bij_auth L ∗*)
-      (*[∗ set] p ∈ L,*)
-        (*let '(b_t, b_s) := p in alloc_unq_rel val_rel b_t b_s pid ∨ alloc_shr_rel val_rel b_t b_s pid)%I.*)
-(*End definitions.*)
-
 Section state_interp.
-  Context `{bor_stateG Σ}.
+  Context `{bor_stateG Σ} (sc_rel : scalar → scalar → iProp Σ).
 
   (* We generally do not enforce that stacks for all locations are equal: that would make non-determinism in choosing locations slightly clunky.
     Rather, we should again force equality in bijections.
   *)
-  Definition bor_interp sc_rel (σ_t : state) (σ_s : state) : iProp Σ :=
-  (* since multiple parts of the interpretation need access to these maps, we own the authoritative parts here and not in the interpretation below *)
-   ∃ (M_call_s M_call_t : gmap call_id (gmap ptr_id (gset loc)))
-     (M_tag : gmap ptr_id (tag_kind * option unit))
-     (M_t M_s : gmap (ptr_id * loc) scalar),
+  Definition bor_auth (M_call_s M_call_t : gmap call_id (gmap ptr_id (gset loc))) (M_tag : gmap ptr_id (tag_kind * unit)) (M_t M_s : gmap (ptr_id * loc) scalar) (L : gset (block * block)) : iProp Σ := 
     ghost_map_auth call_source_name 1 M_call_s ∗
     ghost_map_auth call_target_name 1 M_call_t ∗
     tkmap_auth tag_name 1 M_tag ∗
     ghost_map_auth heap_view_target_name 1 M_t ∗
     ghost_map_auth heap_view_source_name 1 M_s ∗
-    
-    call_set_interp M_call_s σ_s ∗
-    call_set_interp M_call_t σ_t ∗
-    tag_interp sc_rel M_tag M_t M_s σ_t σ_s ∗
+    gset_bij_own_auth heap_bij_name (DfracOwn 1) L.
+  Definition bor_interp (σ_t : state) (σ_s : state) : iProp Σ :=
+  (* since multiple parts of the interpretation need access to these maps, we own the authoritative parts here and not in the interpretations below *)
+   ∃ (M_call_s M_call_t : gmap call_id (gmap ptr_id (gset loc)))
+     (M_tag : gmap ptr_id (tag_kind * unit))
+     (M_t M_s : gmap (ptr_id * loc) scalar) 
+     (L : gset (block * block)),
+    bor_auth M_call_s M_call_t M_tag M_t M_s L ∗
 
-    (*heap_interp heap_source_name σ_s ∗ *)
-    (*heap_interp heap_target_name σ_t ∗*)
+    heap_bij_interp sc_rel M_tag M_t M_call_t L σ_t σ_s ∗
+    ⌜call_set_interp M_call_s σ_s⌝ ∗
+    ⌜call_set_interp M_call_t σ_t⌝ ∗
+    ⌜tag_interp M_tag M_t M_s σ_t σ_s⌝ ∗
 
     (* TODO: for the future, it would be nice to generalize that to a bijection, too *)
     ⌜σ_s.(snp) = σ_t.(snp)⌝ ∗
@@ -342,16 +632,13 @@ Section state_interp.
     ⌜state_wf σ_s⌝ ∗
     ⌜state_wf σ_t⌝.
 
-  Lemma bor_interp_get_pure sc_rel σ_t σ_s :
-    bor_interp sc_rel σ_t σ_s -∗ ⌜σ_s.(snp) = σ_t.(snp) ∧ σ_s.(snc) = σ_t.(snc) ∧ σ_s.(scs) = σ_t.(scs) ∧ state_wf σ_s ∧ state_wf σ_t⌝.
-  Proof. iIntros "(_&_&_&%)". eauto. Qed.
-
+  Lemma bor_interp_get_pure σ_t σ_s :
+    bor_interp σ_t σ_s -∗ ⌜σ_s.(snp) = σ_t.(snp) ∧ σ_s.(snc) = σ_t.(snc) ∧ σ_s.(scs) = σ_t.(scs) ∧ state_wf σ_s ∧ state_wf σ_t⌝.
+  Proof. iIntros "(% & % & % & % & % & %& ? & ? & ? & ? & ? & %)". eauto. Qed.
 End state_interp.
 
 
 (** Array generalizes pointsto connectives to lists of scalars *)
-(*Definition array_local `{!bor_stateG Σ} γh (l : loc) (scts : list (scalar * stack)) : iProp Σ :=*)
-  (*([∗ list] i ↦ sct ∈ scts, heap_pointsto γh (l +ₗ i) sct.1 sct.2)%I.*)
 Definition array_tag `{!bor_stateG Σ} γh (t : ptr_id) (l : loc) (dq : dfrac) (scs : list scalar) : iProp Σ :=
   ([∗ list] i ↦ sc ∈ scs, ghost_map_elem γh (t, l +ₗ i) dq sc)%I.
 
@@ -368,56 +655,12 @@ Notation "l '↦t∗[pub]{' t } scs" := (array_tag heap_view_target_name t l (Df
 Notation "l '↦s∗[pub]{' t } scs" := (array_tag heap_view_source_name t l (DfracDiscarded) scs)
   (at level 20, format "l  ↦s∗[pub]{ t }  scs") : bi_scope.
 
-(*Notation "l '↦t∗' scts" := (array_local heap_target_name l scts)*)
-  (*(at level 20, format "l  ↦t∗  scts") : bi_scope.*)
-(*Notation "l '↦s∗' scts" := (array_local heap_source_name l scts)*)
-  (*(at level 20, format "l  ↦s∗  scts") : bi_scope.*)
-
-Fixpoint heap_array (l : loc) (scs : list scalar) : gmap loc scalar :=
-  match scs with
-  | [] => ∅
-  | sc :: scs' => {[l := sc]} ∪ heap_array (l +ₗ 1) scs'
-  end.
-
-Lemma heap_array_singleton l sc : heap_array l [sc] = {[l := sc]}.
-Proof. by rewrite /heap_array right_id. Qed.
-
-Lemma heap_array_lookup l scs sc k :
-  heap_array l scs !! k = Some sc ↔
-  ∃ j, (0 ≤ j)%Z ∧ k = l +ₗ j ∧ scs !! (Z.to_nat j) = Some sc.
-Proof.
-  revert k l; induction scs as [|sc' scs IH]=> l' l /=.
-  { rewrite lookup_empty. naive_solver lia. }
-  rewrite -insert_union_singleton_l lookup_insert_Some IH. split.
-  - intros [[-> ->] | (Hl & j & ? & -> & ?)].
-    { eexists 0. rewrite shift_loc_0. naive_solver lia. }
-    eexists (1 + j)%Z. rewrite shift_loc_assoc !Z.add_1_l Z2Nat.inj_succ; auto with lia.
-  - intros (j & ? & -> & Hil). destruct (decide (j = 0)); simplify_eq/=.
-    { rewrite shift_loc_0; eauto. }
-    right. split.
-    { rewrite -{1}(shift_loc_0 l). intros ?%(inj (shift_loc _)); lia. }
-    assert (Z.to_nat j = S (Z.to_nat (j - 1))) as Hj.
-    { rewrite -Z2Nat.inj_succ; last lia. f_equal; lia. }
-    rewrite Hj /= in Hil.
-    eexists (j - 1)%Z. rewrite shift_loc_assoc Z.add_sub_assoc Z.add_simpl_l.
-    auto with lia.
-Qed.
-
-Lemma heap_array_map_disjoint (h : gmap loc scalar) (l : loc) (scs : list scalar) :
-  (∀ i, (0 ≤ i)%Z → (i < length scs)%Z → h !! (l +ₗ i) = None) →
-  (heap_array l scs) ##ₘ h.
-Proof.
-  intros Hdisj. apply map_disjoint_spec=> l' v1 v2.
-  intros (j&?&->&Hj%lookup_lt_Some%inj_lt)%heap_array_lookup.
-  move: Hj. rewrite Z2Nat.id // => ?. by rewrite Hdisj.
-Qed.
-
 (** Lemmas / Accessors *)
 Add Printing Constructor state item.
 Section lemmas.
   Context `{bor_stateG Σ} (sc_rel : scalar → scalar → iProp Σ)
     (sc_rel_pers : ∀ sc_t sc_s, Persistent (sc_rel sc_t sc_s)).
-  Notation bor_interp := (bor_interp sc_rel).
+  Local Notation bor_interp := (bor_interp sc_rel).
 
   Implicit Types
     (l : loc) (sc : scalar).
@@ -427,14 +670,14 @@ Section lemmas.
     let l_t := (fresh_block σ_t.(shp), 0) in
     let l_s := (fresh_block σ_s.(shp), 0) in
     let t := σ_t.(snp) in
-    bor_interp
+    bor_interp 
       (mkState (init_mem l_t (tsize T) σ_t.(shp)) (init_stacks σ_t.(sst) l_t (tsize T) (Tagged σ_t.(snp))) σ_t.(scs) (S σ_t.(snp)) σ_t.(snc))
       (mkState (init_mem l_s (tsize T) σ_s.(shp)) (init_stacks σ_s.(sst) l_s (tsize T) (Tagged σ_s.(snp))) σ_s.(scs) (S σ_s.(snp)) σ_s.(snc)) ∗
-      t -->[tk_local] (Some ()) ∗
+      t @@ tk_local ∗
       l_t ↦t∗[local]{t} repeat ScPoison (tsize T) ∗
       l_s ↦s∗[local]{t} repeat ScPoison (tsize T).
   Proof.
-    iIntros "(? & ? & Htag & %Hsnp & %Hsnc & %Hscs & %Hwf_s & %Hwf_t)".
+    iIntros "(% & % & % & % & % & % & ? & Hbij & ? & ? & Htag & %Hsnp & %Hsnc & %Hscs & %Hwf_s & %Hwf_t)".
     (* 1. allocate new local locations
        2. profit
     *)
@@ -469,7 +712,7 @@ Section lemmas.
   Lemma heap_local_access_target σ_t σ_s (t : ptr_id) l  sc :
     bor_interp σ_t σ_s -∗
     l ↦t[local]{t} sc -∗
-    t -->[tk_local] (Some tt) -∗
+    t @@ tk_local -∗
     ⌜σ_t.(shp) !! l = Some sc⌝ ∗
     ⌜σ_t.(sst) !! l = Some [mkItem Unique (Tagged t) None]⌝ ∗
     ⌜wf_scalar σ_t sc⌝ ∗
@@ -480,16 +723,14 @@ Section lemmas.
       bor_interp (state_upd_mem (<[l := sc']>) σ_t) σ_s ∗
       l ↦t[local]{t} sc').
   Proof.
-    iIntros "(Hc_t & Hc_s & Htag_auth & %Hsnp & %Hsnc & %Hscs & %Hwf_s & %Hwf_t)".
+    iIntros "(% & % & % & % & % & % & (Hc_t & ? & Htag_auth & Htag_t_auth & Htag_s_auth & Hbij_auth) & Hbij & ? & ? & %Htag_interp & %Hsnp & %Hsnc & %Hscs & %Hwf_s & %Hwf_t)".
     iIntros "Hp Htag".
-    iDestruct "Htag_auth" as (M_tag Mtag_t Mtag_s) "(Htag_auth & Htag_t_auth & Htag_s_auth & #H)".
     iPoseProof (tkmap_lookup with "Htag_auth Htag") as "%Htag_lookup".
-    iDestruct ("H" with "[//]") as "(_ & _ & Ha)".
-    iDestruct "Ha" as (lb_t lb_s len) "(_ & Ha & %Ht & _)".
+    destruct (Htag_interp _ _ Htag_lookup) as (_ & _ & Ha).
+    destruct Ha as (lb_t & lb_s & len & Ha & Ht & _).
     iPoseProof (ghost_map_lookup with "Htag_t_auth Hp") as "%Ht_lookup".
     specialize (Ht _ _ Ht_lookup) as (o & -> & Ho).
-    iDestruct ("Ha" $! o with "[//]") as (sc_t sc_s) "(%Hcontrol & _)".
-    destruct Hcontrol as (Ht_lookup' & Hcontrol & _ & _).
+    destruct (Ha o ltac:(lia)) as (sc_t & sc_s & Ht_lookup' & Hcontrol & _).
     rewrite Ht_lookup in Ht_lookup'. injection Ht_lookup' as [= <-].
     specialize (loc_controlled_local _ _ _ _ Hcontrol) as (Hstack & Hmem).
     iSplitR; first done. iSplitR; first done.
@@ -501,23 +742,26 @@ Section lemmas.
     iIntros (sc') "%Hwf_sc".
     iMod (ghost_map_update sc' with "Htag_t_auth Hp") as "[Htag_t_auth $]".
     iModIntro. rewrite /bor_interp.
-    iFrame "Hc_t Hc_s". cbn. iSplitL; first last.
+    iExists M_call_s, M_call_t, M_tag, (<[(t, lb_t +ₗ o):=sc']> M_t), M_s, L.
+    iFrame. cbn. iSplitL "Hbij". 
+    { iApply (heap_bij_interp_update_private_target with "Hbij"). 
+      - eauto. 
+      - exists tk_local. split_and!; [done | by eauto | by left ].
+    } 
+    iSplitR; first last.
     { repeat iSplitL; [ done.. | ].
       iPureIntro. apply state_wf_upd_mem; [by eauto | done | done].
     } 
-    iExists M_tag, (<[(t, lb_t +ₗ o):=sc']> Mtag_t), Mtag_s.
-    iFrame. iClear "Ha Htag". clear lb_s sc_s.
+    clear Ha lb_s sc_s.
 
-    iIntros (t' tk' ol') "%Hlookup". iDestruct ("H" with "[//]") as "(? & ? & H')".
-    do 2 (iSplitR; first done).
-    iDestruct "H'" as (lb_t' lb_s' len') "(-> & Hoo & %Ha_t & %Ha_s)".
-    iExists lb_t', lb_s', len'. iSplitR; first done.
-    iSplitL; last iSplit; last done.
-    - iIntros (o') "%Ho'". iDestruct ("Hoo" with "[//]") as (sc_t sc_s) "[%Hoo Hsc]".
-      iClear "Hoo".
+    iPureIntro.
+    intros t' tk' (? & ? & H')%Htag_interp. do 2 (split; first done).
+    destruct H' as (lb_t' & lb_s' & len' & Hoo & Ha_t & Ha_s).
+    exists lb_t', lb_s', len'. 
+    split_and!; last done.
+    - intros o' Ho'. specialize (Hoo _ Ho') as (sc_t & sc_s & Hoo). 
       destruct (decide (t = t')) as [<- | Hneq]; first last.
-      { iExists sc_t, sc_s. rewrite lookup_insert_ne; last congruence.
-        iSplitR; last iApply "Hsc". iPureIntro. 
+      { exists sc_t, sc_s. rewrite lookup_insert_ne; last congruence.
         split_and!; [ apply Hoo | | apply Hoo..].  
         destruct (decide (lb_t' +ₗ o' = lb_t +ₗ o)) as [-> | Hneq_loc].
         { (* this is contradictory, as tag t has local ownership *)
@@ -525,24 +769,22 @@ Section lemmas.
         } 
         apply loc_controlled_mem_insert_ne; [done | apply Hoo]. 
       } 
-      rewrite Htag_lookup in Hlookup. injection Hlookup as [= <-].
-      destruct (decide (lb_t' +ₗ o' = lb_t +ₗ o)) as [-> | Hneq_loc].
-      + iExists sc', sc_s. iSplit; last (iIntros "%"; congruence).
-        iPureIntro. 
+      revert Hoo.
+      destruct (decide (lb_t' +ₗ o' = lb_t +ₗ o)) as [-> | Hneq_loc] => Hoo.
+      + exists sc', sc_s.
         rewrite lookup_insert. split_and!; [ done | | apply Hoo..].  
-        eapply loc_controlled_mem_insert; done.
-      + iExists sc_t, sc_s. iSplit; last (iIntros "%"; congruence).
-        iPureIntro. 
+        eapply loc_controlled_mem_insert, Hoo.
+      + exists sc_t, sc_s.
         rewrite lookup_insert_ne; last congruence. 
         split_and!; [ apply Hoo | | apply Hoo..].  
         eapply loc_controlled_mem_insert_ne; [done | apply Hoo].
-    - iPureIntro. (* easy *) admit.
+    - (* easy *) admit.
   Admitted. 
 
   Lemma heap_local_accessN_target' σ_t σ_s (t : ptr_id) l scs :
     bor_interp σ_t σ_s -∗
     l ↦t∗[local]{t} scs -∗
-    t -->[tk_local] (Some tt) -∗
+    t @@ tk_local -∗
     ⌜∀ i : nat, i < length scs → σ_t.(shp) !! (l +ₗ i) = scs !! i ⌝ ∗
     ⌜∀ i, i < length scs → σ_t.(sst) !! (l +ₗ i) = Some [mkItem Unique (Tagged t) None]⌝ ∗
     (∀ scs',
@@ -558,7 +800,7 @@ Section lemmas.
   Lemma heap_local_accessN_target σ_t σ_s (t : ptr_id) l scs :
     bor_interp σ_t σ_s -∗
     l ↦t∗[local]{t} scs -∗
-    t -->[tk_local] (Some tt) -∗
+    t @@ tk_local -∗
     ⌜read_mem l (length scs) σ_t.(shp) = Some scs⌝ ∗
     ⌜∀ i, i < length scs → σ_t.(sst) !! (l +ₗ i) = Some [mkItem Unique (Tagged t) None]⌝ ∗
     ⌜scs <<t σ_t.(snp)⌝ ∗
@@ -572,26 +814,26 @@ Section lemmas.
   Proof.
   Admitted.
 
-  Lemma heap_local_access_source σ_t σ_s (t : ptr_id) l  sc :
+  Lemma heap_local_access_source σ_t σ_s (t : ptr_id) l sc :
     bor_interp σ_t σ_s -∗
     l ↦s[local]{t} sc -∗
-    t -->[tk_local] (Some tt) -∗
+    t @@ tk_local -∗
     ⌜σ_s.(shp) !! l = Some sc⌝ ∗
     ⌜σ_s.(sst) !! l = Some [mkItem Unique (Tagged t) None]⌝ ∗
     ⌜wf_scalar σ_s sc⌝ ∗
     (∀ sc',
-      ⌜wf_scalar σ_t sc' ⌝ -∗
+      ⌜wf_scalar σ_s sc' ⌝ -∗
       (*stack_wf st' σ_t -∗ *)
       |==>
       bor_interp σ_t (state_upd_mem (<[l := sc']>) σ_s) ∗
       l ↦s[local]{t} sc').
   Proof.
-  Admitted. 
+  Admitted.
 
   Lemma heap_local_accessN_source σ_t σ_s (t : ptr_id) l scs :
     bor_interp σ_t σ_s -∗
     l ↦s∗[local]{t} scs -∗
-    t -->[tk_local] (Some tt) -∗
+    t @@ tk_local -∗
     ⌜read_mem l (length scs) σ_s.(shp) = Some scs⌝ ∗
     ⌜∀ i, i < length scs → σ_s.(sst) !! (l +ₗ i) = Some [mkItem Unique (Tagged t) None]⌝ ∗
     ⌜scs <<t σ_s.(snp)⌝ ∗
@@ -616,7 +858,7 @@ End lemmas.
 
 
 
-
+(* NOTE: might need to generalize that with the bijection a bit when we want to do cool things, e.g., pass parts of an object to a function (but for just obtaining a reflexivity thm, it should be fine) *)
 Section val_rel.
   Context {Σ} `{bor_stateG Σ}.
   Fixpoint sc_rel (sc1 sc2 : scalar) {struct sc2} : iProp Σ :=
@@ -624,11 +866,13 @@ Section val_rel.
     | ScInt z1, ScInt z2 => ⌜z1 = z2⌝
     | ScFnPtr f1, ScFnPtr f2 => ⌜f1  = f2⌝
     | ScPtr l1 t1, ScPtr l2 t2 =>
-        (⌜t1 = Untagged⌝ ∗ ⌜t2 = Untagged⌝ (* TODO: probably need somethng more here *)) ∨
+        (* asserts that: the stacks are the same, the allocation size is the same, and that the locations are related *)
+        l1 ↔h l2 ∗
+        (⌜t1 = Untagged⌝ ∗ ⌜t2 = Untagged⌝) ∨
         (∃ p1 p2, ⌜t1 = Tagged p1⌝ ∗ ⌜t2 = Tagged p2⌝ ∗
-        (* TODO: may want to generalize that properly when we have a proper bijection on tags*)
+        (* may want to generalize that properly when we have a proper bijection on tags*)
         ⌜p2 = p1⌝ ∗
-        p1 -->[tk_pub] (Some tt)
+        p1 @@ tk_pub
         (* note: we do not have any assertion about the value as viewed by the tag here -- we don't really care about it, we need to do a retag anyways *)
       )
     | _, _ => False
@@ -637,7 +881,7 @@ Section val_rel.
   Global Instance sc_rel_persistent sc_t sc_s : Persistent (sc_rel sc_t sc_s).
   Proof. destruct sc_t, sc_s; apply _. Qed.
 
-  (*Definition val_rel (v1 v2 : value) *)
+  (*Definition value_rel (v1 v2 : value) := Forall2*)
 End val_rel.
 
 Class sborG (Σ: gFunctors) := SBorG {
@@ -645,13 +889,15 @@ Class sborG (Σ: gFunctors) := SBorG {
   sborG_stateG :> bor_stateG Σ;
 }.
 
-Global Instance sborG_SimulLang `{!sborG Σ} : SimulLang (iPropI Σ) bor_lang := {
-  state_interp P_t σ_t P_s σ_s :=
+Global Program Instance sborG_simulirisG `{!sborG Σ} : simulirisG (iPropI Σ) bor_lang := {
+  state_interp P_t σ_t P_s σ_s T_s :=
     (gen_prog_interp (hG := gen_prog_inG_target) P_t ∗
      gen_prog_interp (hG := gen_prog_inG_source) P_s ∗
      bor_interp sc_rel σ_t σ_s
     )%I;
 }.
+Next Obligation.
+Admitted.
 
 
 Section lifting.
@@ -664,25 +910,21 @@ Implicit Types l : loc.
 Implicit Types f : fname.
 
 Context (Ω : result → result → iProp Σ).
-Local Notation "et '⪯' es [{ Φ }]" := (et ⪯{Ω} es [{Φ}])%I (at level 40, Φ at level 200) : bi_scope.
-Local Notation "et '⪯' es {{ Φ }}" := (et ⪯{Ω} es {{Φ}})%I (at level 40, Φ at level 200) : bi_scope.
 
-(*Definition as_local (scs : list scalar) t := map (λ sc, (sc, [mkItem Unique (Tagged t) None])) scs.*)
-(*Lemma as_local_const sc n t :*)
-  (*as_local (repeat sc n) t = repeat (sc, [mkItem Unique (Tagged t) None]) n.*)
-(*Proof.*)
-  (*induction n as [ | n IH]; cbn; first done. by rewrite -IH.*)
-(*Qed.*)
+Lemma fresh_block_det σ_s σ_t : 
+  dom (gset loc) σ_s.(shp) = dom (gset loc) σ_t.(shp) →
+  fresh_block σ_s.(shp) = fresh_block σ_t.(shp).
+Proof. rewrite /fresh_block. intros ->. done. Qed.
 
-Lemma sim_alloc T Φ :
-  (∀ t l_t l_s, t -->[tk_local] Some () -∗
+Lemma sim_alloc T Φ π :
+  (∀ t l_t l_s, t @@ tk_local -∗
     l_t ↦t∗[local]{t} repeat ScPoison (tsize T) -∗
     l_s ↦s∗[local]{t} repeat ScPoison (tsize T) -∗
-    Place l_t (Tagged t) T ⪯ Place l_s (Tagged t) T {{ Φ }}) -∗
-  Alloc T ⪯ Alloc T {{ Φ }}.
+    Place l_t (Tagged t) T ⪯{π, Ω} Place l_s (Tagged t) T {{ Φ }}) -∗
+  Alloc T ⪯{π, Ω} Alloc T {{ Φ }}.
 Proof.
   iIntros "Hsim".
-  iApply sim_lift_head_step_both. iIntros (????) "[(HP_t & HP_s & Hbor) %Hnreach]".
+  iApply sim_lift_head_step_both. iIntros (??????) "[(HP_t & HP_s & Hbor) %Hsafe]".
   iPoseProof (bor_interp_get_pure with "Hbor") as "%Hp".
   iModIntro. iSplitR.
   { iPureIntro. do 3 eexists. econstructor 2; econstructor. }
@@ -698,15 +940,21 @@ Proof.
   iApply ("Hsim" with "Htag Htarget Hsource").
 Qed.
 
+(*Lemma sim_make_public T Φ π : *)
+  (*t @@ tk_local -∗ *)
+  (*l_t ↦t∗[local]{t} repeat ScPoison (tsize T) -∗*)
+  (*l_s ↦s∗[local]{t} repeat ScPoison (tsize T) -∗*)
+
+
 Lemma target_local_copy scs T l t Ψ :
   length scs = tsize T →
-  t -->[tk_local] Some tt -∗ 
+  t @@ tk_local -∗ 
   l ↦t∗[local]{t} scs -∗
   (l ↦t∗[local]{t} scs -∗ target_red #scs Ψ)%E -∗
   target_red (Copy (Place l (Tagged t) T)) Ψ.
 Proof.
   iIntros (Hlen) "Htag Ht Hsim".
-  iApply target_red_lift_head_step. iIntros (????) "(HP_t & HP_s & Hbor)".
+  iApply target_red_lift_head_step. iIntros (?????) "(HP_t & HP_s & Hbor)".
   iModIntro. 
   iPoseProof (heap_local_accessN_target with "Hbor Ht Htag") as "(%Hd & %Hstack & %Hwf & Hclose)".
   iSplitR.
@@ -729,15 +977,15 @@ Proof.
   admit. 
 Admitted.
 
-Lemma source_local_copy scs T l t Ψ :
+Lemma source_local_copy scs T l t Ψ π :
   length scs = tsize T →
-  t -->[tk_local] Some tt -∗ 
+  t @@ tk_local -∗ 
   l ↦s∗[local]{t} scs -∗
-  (l ↦s∗[local]{t} scs -∗ source_red #scs Ψ)%E -∗
-  source_red (Copy (Place l (Tagged t) T)) Ψ.
+  (l ↦s∗[local]{t} scs -∗ source_red #scs π Ψ)%E -∗
+  source_red (Copy (Place l (Tagged t) T)) π Ψ.
 Proof.
   iIntros (Hlen) "Htag Hs Hsim".
-  iApply source_red_lift_head_step. iIntros (????) "[(HP_t & HP_s & Hbor) _]".
+  iApply source_red_lift_head_step. iIntros (??????) "[(HP_t & HP_s & Hbor) _]".
   iModIntro. 
   iPoseProof (heap_local_accessN_source with "Hbor Hs Htag") as "(%Hd & %Hstack & %Hwf & Hclose)".
   assert (head_reducible P_t (Copy (Place l (Tagged t) T)) σ_s) as (e_s' & σ_s' & efs & Hstep).
@@ -760,11 +1008,12 @@ Proof.
   admit. 
 Admitted.
 
-Lemma sim_retag_default_mutref l_t l_s ot Φ c pkind T : 
-  (∀ nt, t -->[tk_local] #[ScPtr l_t nt] ⪯ #[ScPtr l_s nt] [{ Φ }]) -∗
-  Retag #[ScPtr l_t ot] #[ScCallId c] (RefPtr Mutable) T Default ⪯ Retag #[ScPtr l_s ot] #[ScCallId c] (RefPtr Mutable) T Default [{ Φ }].
-Proof. 
+(*Lemma sim_retag_default_mutref l_t l_s ot Φ c pkind T π : *)
+  (*(∀ nt, nt @@ tk_local -∗ #[ScPtr l_t nt] ⪯{π, Ω} #[ScPtr l_s nt] [{ Φ }]) -∗*)
+  (*Retag #[ScPtr l_t ot] #[ScCallId c] (RefPtr Mutable) T Default ⪯{π, Ω} Retag #[ScPtr l_s ot] #[ScCallId c] (RefPtr Mutable) T Default [{ Φ }].*)
+(*Proof. *)
 
+(*Abort.*)
 
 
 
